Finish correctness proof, add intro rules, start example usage

Steps.thy
@@ -36,6 +36,8 @@ fun n_steps :: "flow_state \<Rightarrow> nat \<Rightarrow> flow_state \<Rightarr
 
 notation n_steps ("(_ \<rightarrow>^_ _)" [51, 0, 51] 50)
 
+find_consts name: tranc
+
 lemma steps_exists_n_steps:
   assumes "fs \<rightarrow>* fs'"
   shows "\<exists>n. fs \<rightarrow>^n fs'"
@@ -71,6 +73,8 @@ lemma step_models_execute_blocks_ok:
   assumes "terminal_state fs'"
   assumes "fs = bbranch s prev lab"
   assumes "\<not> is_berr fs'"
+  assumes "fs \<rightarrow>* fs'"
+  assumes "terminal_state fs'"
   shows   "execute_blocks prev lab (llvm_function.blocks f) s = ok (state fs', ret_value fs')"
   using assms
   apply (induction arbitrary: s prev lab rule: converse_rtranclp_induct)
@@ -89,16 +93,19 @@ lemma step_models_execute_blocks_err:
   by (subst execute_blocks.simps; auto split: option.splits result.splits llvm_block_return.splits simp: step_def)
 
 
-definition "wp_steps fs Q \<equiv> \<forall>fs'. fs \<rightarrow>* fs' \<and> terminal_state fs' \<longrightarrow> \<not>is_berr fs' \<and> Q (state fs') (ret_value fs')"
+definition "wp_steps fs Q \<equiv> \<forall>fs'. fs \<rightarrow>* fs' \<and> terminal_state fs' \<longrightarrow> (\<not>is_berr fs') \<and> (Q (state fs') (ret_value fs'))"
 
 
 type_synonym precondition  = "state \<Rightarrow> bool"
-type_synonym preconditions = "llvm_identifier option \<Rightarrow> llvm_identifier \<Rightarrow> precondition option"
+type_synonym preconditions = "((llvm_identifier option * llvm_identifier) * precondition) list"
 type_synonym postcondition = "state \<Rightarrow> llvm_value option \<Rightarrow> bool"
 
+fun predicate_for_all where
+  "predicate_for_all P [] = True"
+| "predicate_for_all P (((p,l),pre)#pres) = (P p l \<and> predicate_for_all P pres)"
 
 context
-  fixes annotations :: "llvm_identifier option \<Rightarrow> llvm_identifier \<Rightarrow> precondition option"
+  fixes annotations :: "preconditions"
   fixes post :: "postcondition"
 begin
 
@@ -114,7 +121,7 @@ definition "has_annotation fs \<equiv>
   (case fs of
     berr \<Rightarrow> False
   | bret _ _ \<Rightarrow> True
-  | bbranch _ p l \<Rightarrow> (annotations p l) \<noteq> None
+  | bbranch _ p l \<Rightarrow> map_of annotations (p,l) \<noteq> None
   )"
 
 definition "annotation_holds fs \<equiv>
@@ -122,125 +129,191 @@ definition "annotation_holds fs \<equiv>
     berr \<Rightarrow> False
   | bret s v \<Rightarrow> post s v
   | bbranch s p l \<Rightarrow> has_annotation fs \<and>
-    (case (annotations p l) of
+    (case map_of annotations (p,l) of
       None \<Rightarrow> False
     | Some annot \<Rightarrow> annot s
     )
   )"
 
-definition step_until :: "flow_state \<Rightarrow> flow_state \<Rightarrow> bool" (infix "\<Rightarrow>" 50) where
+
+definition step_until :: "flow_state \<Rightarrow> flow_state \<Rightarrow> bool" where
   "step_until fs fs' \<equiv> step fs fs' \<and> \<not>has_annotation fs"
-abbreviation steps_until :: "flow_state \<Rightarrow> flow_state \<Rightarrow> bool" (infix "\<Rightarrow>*" 50) where
-  "fs \<Rightarrow>* fs' \<equiv> step_until\<^sup>*\<^sup>* fs fs'"
 
-fun n_steps_until :: "flow_state \<Rightarrow> nat \<Rightarrow> flow_state \<Rightarrow> bool" where
-  "n_steps_until s 0 s'  = (s = s')"
-| "n_steps_until s (Suc n) s' = (\<exists>x. s \<Rightarrow> x \<and> n_steps_until x n s')"
-
-notation n_steps_until ("(_ \<Rightarrow>^_ _)" [51, 0, 51] 50)
-
-definition keep_stepping_until :: "flow_state \<Rightarrow> flow_state \<Rightarrow> bool" (infix "\<Rightarrow>*a" 50) where
-  "keep_stepping_until s s' \<equiv> (\<exists>x. s \<rightarrow> x \<and> x \<Rightarrow>* s') \<and> (has_annotation s')"
-abbreviation keep_stepping_until_closure :: "flow_state \<Rightarrow> flow_state \<Rightarrow> bool" (infix "\<Rightarrow>*a*" 50) where
-  "fs \<Rightarrow>*a* fs' \<equiv> keep_stepping_until\<^sup>*\<^sup>* fs fs'"
+definition annotated_step :: "flow_state \<Rightarrow> flow_state \<Rightarrow> bool" (infix "\<Rightarrow>" 50) where
+  "annotated_step s s' \<equiv> (\<exists>x. s \<rightarrow> x \<and> step_until\<^sup>*\<^sup>* x s') \<and> (has_annotation s' \<or> is_berr s')"
+abbreviation annotated_steps :: "flow_state \<Rightarrow> flow_state \<Rightarrow> bool" (infix "\<Rightarrow>*" 50) where
+  "fs \<Rightarrow>* fs' \<equiv> annotated_step\<^sup>*\<^sup>* fs fs'"
 
 
-lemma annotation_simps[simp]:
-  "\<nexists>fs'. step_until fs fs' \<Longrightarrow> \<not>is_berr fs \<Longrightarrow> has_annotation fs"
-  "annotations p l \<noteq> None \<Longrightarrow> \<forall>s. has_annotation (bbranch s p l)"
-  unfolding step_until_def has_annotation_def step_def
-  by (auto split: flow_state.splits)
 
-lemma step_until_single[simp]:
-  "\<nexists>fs' fs''. step_until fs fs' \<and> step_until fs fs'' \<and> fs' \<noteq> fs''"
-  unfolding step_until_def step_def by blast
+definition wp_step where
+  "wp_step fs Q \<equiv> (\<forall>fs'. step fs fs' \<longrightarrow> \<not>is_berr fs' \<and> Q fs')"
 
-lemma steps_until_models_steps:
-  assumes "fs \<Rightarrow>* fs'"
-  shows "fs \<rightarrow>* fs'"
+definition wp_steps_until where
+  "wp_steps_until fs Q \<equiv> (\<forall>fs'. (step_until)\<^sup>*\<^sup>* fs fs' \<and> \<not>is_berr fs \<longrightarrow> \<not>is_berr fs') \<and> (\<forall>fs'. (step_until)\<^sup>*\<^sup>* fs fs' \<and> has_annotation fs' \<longrightarrow> Q fs')"
+
+definition wp_annotated_step where
+  "wp_annotated_step fs Q \<equiv> (\<forall>fs'. annotated_step fs fs' \<longrightarrow> \<not>is_berr fs' \<and> Q fs')"
+
+lemma wp_step_intro:
+  assumes "map_of (llvm_function.blocks f) l = Some b"
+  assumes "wp (execute_block p b s) (\<lambda>(s', r). case r of branch_label l' \<Rightarrow> Q (bbranch s' (Some l) l') | return_value v \<Rightarrow> Q (bret s' (Some v)))"
+  shows "wp_step (bbranch s p l) Q"
   using assms
-  unfolding step_until_def
-  apply (induction rule: rtranclp_induct)
-  by auto
+  unfolding wp_step_def wp_gen_def step_def
+  by (auto split: result.splits llvm_block_return.splits)
 
-lemma keep_stepping_until_models_steps:
-  assumes "fs \<Rightarrow>*a fs'"
-  shows "fs \<rightarrow>* fs'"
-  using assms steps_until_models_steps
-  unfolding keep_stepping_until_def
-  by fastforce
+lemma wp_steps_until_intro:
+  assumes "has_annotation fs \<Longrightarrow> Q fs"
+  assumes "\<not>has_annotation fs \<Longrightarrow> wp_step  fs (\<lambda>fs'. wp_steps_until fs' Q)"
+  shows "wp_steps_until fs Q"
+  using assms converse_rtranclpE step_until_def
+  unfolding wp_steps_until_def wp_step_def
+  by metis
 
-lemma keep_stepping_impl_has_annotation:
-  assumes "fs \<Rightarrow>*a fs'"
-  shows "has_annotation fs'"
+lemma wp_annotated_step_intro:
+  assumes "wp_step fs (\<lambda>fs'. wp_steps_until fs' Q)"
+  shows "wp_annotated_step fs Q"
   using assms
-  unfolding keep_stepping_until_def
+  unfolding wp_annotated_step_def wp_step_def annotated_step_def wp_steps_until_def
   by blast
 
 
-definition "floyd_cond s p l \<equiv> \<forall>fs'.
-    (bbranch s p l) \<Rightarrow>*a fs'
-    \<longrightarrow> \<not>is_berr fs' \<and> annotation_holds fs'"
+
+definition "floyd_cond s p l \<equiv> wp_annotated_step (bbranch s p l) (\<lambda>fs'. annotation_holds fs')"
+
 
 definition floyd_vc :: "bool" where
   "floyd_vc \<equiv>
-    annotations None first_label \<noteq> None
-    \<and> (\<exists>s. annotation_holds (bbranch s None first_label))
-    \<and> (\<forall>p l. annotations p l \<noteq> None \<longrightarrow> (\<forall>s. annotation_holds (bbranch s p l) \<longrightarrow> floyd_cond s p l))"
+    map_of annotations (None, first_label) \<noteq> None
+    \<and> (\<forall>p l. map_of annotations (p,l) \<noteq> None \<longrightarrow> (\<forall>s. annotation_holds (bbranch s p l) \<longrightarrow> floyd_cond s p l))"
 
+lemma predicate_for_all_impl_for_all_map_of:
+  assumes "predicate_for_all (\<lambda>p l. (\<forall>s. annotation_holds (bbranch s p l) \<longrightarrow> floyd_cond s p l)) a"
+  shows "(\<forall>p l. map_of a (p,l) \<noteq> None \<longrightarrow> (\<forall>s. annotation_holds (bbranch s p l) \<longrightarrow> floyd_cond s p l))"
+  using assms
+  apply (induction a)
+  subgoal by force
+  subgoal for annot annots
+    apply (intro allI impI)
+    subgoal for p l s
+      apply (cases "annot")
+      subgoal for br pre
+        apply (cases "br = (p,l)")
+        subgoal
+          by (metis (no_types, lifting) predicate_for_all.simps(2))
+        subgoal premises prems
+        proof -
+          have "predicate_for_all (\<lambda>p l. (\<forall>s. annotation_holds (bbranch s p l) \<longrightarrow> floyd_cond s p l)) annots" using prems
+            using predicate_for_all.elims(2) by blast 
+          then show ?thesis
+            by (metis map_of_Cons_code(2) prems(1,3,4,5,6))
+        qed
+        done
+      done
+    done
+  done
+
+lemma floyd_vc_intro:
+  assumes "map_of annotations (None, first_label) \<noteq> None"
+  assumes "predicate_for_all (\<lambda>p l. (\<forall>s. annotation_holds (bbranch s p l) \<longrightarrow> floyd_cond s p l)) annotations"
+  shows "floyd_vc"
+  unfolding floyd_vc_def
+  using predicate_for_all_impl_for_all_map_of assms
+  by blast
 
 lemma floyd_vc_impl_annotation_holds:
   assumes "floyd_vc"
-  shows "\<forall>fs fs'. annotation_holds fs \<and> fs \<Rightarrow>*a fs' \<longrightarrow> annotation_holds fs'"
+  shows "\<forall>fs fs'. annotation_holds fs \<and> fs \<Rightarrow> fs' \<longrightarrow> annotation_holds fs'"
   using assms
-  apply (intro allI impI) subgoal for fs
-  unfolding floyd_vc_def floyd_cond_def has_annotation_def keep_stepping_until_def annotation_holds_def has_annotation_def step_def
-  by (cases fs; fastforce)
-  done
+  unfolding floyd_vc_def floyd_cond_def wp_annotated_step_def has_annotation_def annotated_step_def annotation_holds_def has_annotation_def step_def
+  by (auto split: flow_state.splits; fastforce)
+  
 
-lemma floyd_vc_impl_post_cond:
+
+lemma floyd_vc_impl_annotated_steps_hold:
+  assumes "fs \<Rightarrow>* fs'"
   assumes "floyd_vc"
-  shows "\<forall>fs s v. annotation_holds fs \<and> fs \<Rightarrow>*a bret s v \<longrightarrow> post s v"
-  using assms
-  apply (intro allI impI) subgoal for fs
-  unfolding floyd_vc_def floyd_cond_def has_annotation_def keep_stepping_until_def annotation_holds_def has_annotation_def step_def
-  by (cases fs; fastforce)
-  done
-
-lemma floyd_vc_impl_annotation_holds_for_closure_helper:
-  assumes "fs \<Rightarrow>*a* fs'"
   assumes "annotation_holds fs"
-  assumes "floyd_vc"
   shows "annotation_holds fs'"
   using assms floyd_vc_impl_annotation_holds
-  by (induction rule: rtranclp_induct; blast)
+  by (induction rule: converse_rtranclp_induct; blast)
 
-lemma floyd_vc_impl_annotation_holds_for_closure:
-  assumes "floyd_vc"
-  shows "\<forall>fs fs'. annotation_holds fs \<and> fs \<Rightarrow>*a* fs' \<longrightarrow> annotation_holds fs'"
-  using assms floyd_vc_impl_annotation_holds_for_closure_helper
-  by blast
+lemma exists_first_cutpoint:
+  assumes "fs \<rightarrow>^n fs'"
+  assumes "is_berr fs' \<or> has_annotation fs'"
+  shows "\<exists>fsp m. step_until\<^sup>*\<^sup>* fs fsp \<and> (is_berr fsp \<or> has_annotation fsp) \<and> fsp \<rightarrow>^m fs' \<and> m \<le> n"
+  using assms
+  proof (induction n arbitrary: fs)
+    case 0
+    
+    then show ?case
+      by force
+  next
+    case (Suc n)
+  
+    then show ?case
+      by (smt (verit, ccfv_threshold) n_steps.elims(1) nat.inject nat_le_linear not_less_eq_eq
+          r_into_rtranclp rtranclp.rtrancl_refl rtranclp_trans step_until_def)
+  qed
 
-lemma
-  "fs \<Rightarrow>*a* fs' \<Longrightarrow> fs \<rightarrow>* fs'"
-    apply (induction rule: converse_rtranclp_induct)
-    apply fast
-    using keep_stepping_until_models_steps
-    by force 
+lemma steps_to_annotation_impl_annotated_steps:
+  assumes path: "fs \<rightarrow>* fs'"
+  assumes annot: "has_annotation fs' \<or> is_berr fs'"
+  shows "fs \<Rightarrow>* fs'"
+proof -
+  obtain n where ndef: "fs \<rightarrow>^n fs'" using path steps_exists_n_steps by blast
+  
+  then show ?thesis
+  proof (induction n arbitrary: fs rule: less_induct)
+    case (less n)
+
+    then show ?case
+      proof (cases "n")
+        case 0
+        then show ?thesis
+        using less by fastforce
+      next
+        case (Suc n')
+        then obtain fs1 where fs1def1: "fs \<rightarrow> fs1" and fs1def: "fs1 \<rightarrow>^n' fs'"
+          using less ndef
+          by auto
+      
+        obtain fsa m where "step_until\<^sup>*\<^sup>* fs1 fsa" "has_annotation fsa \<or> is_berr fsa" "fsa \<rightarrow>^m fs'" "m \<le> n'"
+          using fs1def exists_first_cutpoint annot
+          by blast
+
+      then have "fs \<Rightarrow> fsa" using fs1def1 unfolding annotated_step_def by blast
+
+      also from less.IH[OF _ \<open>fsa \<rightarrow>^m fs'\<close>] \<open>m \<le> n'\<close> Suc annot have "fsa \<Rightarrow>* fs'" by force
+      
+      finally show ?thesis .
+      qed
+    qed
+  qed
 
 lemma floyd_vc_impl_wp_step:
   assumes "floyd_vc"
-  assumes "fs = bbranch s None first_label"
   assumes "annotation_holds fs"
+  assumes "fs = bbranch s None first_label"
   shows "wp_steps fs post"
-  using assms
-proof (-)
+  using assms 
+  unfolding floyd_vc_def floyd_cond_def wp_steps_def
+  apply (intro allI impI)
+  apply (elim conjE)
+  subgoal premises prems for fs'
+  proof -
+    have "fs \<Rightarrow>* fs'"
+      using prems steps_to_annotation_impl_annotated_steps
+      unfolding terminal_state_def has_annotation_def is_berr_def
+      by (cases fs'; simp)
 
-  show ?thesis using floyd_vc_impl_post_cond floyd_vc_impl_annotation_holds unfolding wp_steps_def
-    oops
-qed
-  
-
+    then show ?thesis
+      using floyd_vc_impl_annotated_steps_hold assms prems
+      unfolding annotation_holds_def
+      by (cases fs'; fastforce)
+  qed
+  done
 
 end
 
